further cleaning IP Addresses

thy/IP_Addresses/IPv4Addr.thy
@@ -2,30 +2,20 @@
     Authors:    Cornelius Diekmann, Julius Michaelis
 *)
 theory IPv4Addr
-imports Main
-  IPAddr
-  "~~/src/HOL/Library/Code_Target_Nat" (*!*)
+imports IPAddr
+        (* include "~~/src/HOL/Library/Code_Target_Nat" if you need to work with actual numbers.*)
 begin
 
-value "(2::nat) < 2^32" (*without Code_Target_Nat, this would be really slow*)
 
-
-section \<open>Modelling IPv4 Adresses\<close>
-  text\<open>An IPv4 address is basically a 32 bit unsigned integer\<close>
+section \<open>IPv4 Adresses\<close>
+  text\<open>An IPv4 address is basically a 32 bit unsigned integer.\<close>
   type_synonym ipv4addr = "32 word"
- 
-  value "42 :: ipv4addr"
-
-  value "(42 :: ipv4addr) \<le> 45"
 
   text\<open>Conversion between natural numbers and IPv4 adresses\<close>
   definition nat_of_ipv4addr :: "ipv4addr \<Rightarrow> nat" where
     "nat_of_ipv4addr a = unat a"
   definition ipv4addr_of_nat :: "nat \<Rightarrow> ipv4addr" where
     "ipv4addr_of_nat n =  of_nat n"
-
-  lemma "((nat_of_ipv4addr (42::ipv4addr))::nat) = 42" by eval
-  lemma "((ipv4addr_of_nat (42::nat))::ipv4addr) = 42" by eval
 
   text\<open>The maximum IPv4 addres\<close>
   definition max_ipv4_addr :: "ipv4addr" where 
@@ -39,29 +29,19 @@ section \<open>Modelling IPv4 Adresses\<close>
     by(simp add: max_ipv4_addr_number max_word_def)
   lemma max_ipv4_addr_max[simp]: "\<forall>a. a \<le> max_ipv4_addr"
     by(simp add: max_ipv4_addr_max_word)
-  lemma range_0_max_UNIV: "UNIV = {0 .. max_ipv4_addr}" (*not in the simp set, for a reason*)
+  lemma UNIV_ipv4addrset: "UNIV = {0 .. max_ipv4_addr}" (*not in the simp set, for a reason*)
     by(simp add: max_ipv4_addr_max_word) fastforce
 
   text\<open>identity functions\<close>
-  lemma nat_of_ipv4addr_ipv4addr_of_nat: "\<lbrakk> n \<le> nat_of_ipv4addr max_ipv4_addr \<rbrakk> \<Longrightarrow> nat_of_ipv4addr (ipv4addr_of_nat n) = n"
-    by (metis ipv4addr_of_nat_def le_unat_uoi nat_of_ipv4addr_def)
+  lemma nat_of_ipv4addr_ipv4addr_of_nat:
+    "\<lbrakk> n \<le> nat_of_ipv4addr max_ipv4_addr \<rbrakk> \<Longrightarrow> nat_of_ipv4addr (ipv4addr_of_nat n) = n"
+    by (simp add: ipv4addr_of_nat_def le_unat_uoi nat_of_ipv4addr_def)
   lemma nat_of_ipv4addr_ipv4addr_of_nat_mod: "nat_of_ipv4addr (ipv4addr_of_nat n) = n mod 2^32"
     by(simp add: ipv4addr_of_nat_def nat_of_ipv4addr_def unat_of_nat)
   lemma ipv4addr_of_nat_nat_of_ipv4addr: "ipv4addr_of_nat (nat_of_ipv4addr addr) = addr"
     by(simp add: ipv4addr_of_nat_def nat_of_ipv4addr_def)
 
-
-  text\<open>Equality of IPv4 adresses\<close>
-  lemma "\<lbrakk> n \<le> nat_of_ipv4addr max_ipv4_addr \<rbrakk> \<Longrightarrow> nat_of_ipv4addr (ipv4addr_of_nat n) = n"
-    apply(simp add: nat_of_ipv4addr_def ipv4addr_of_nat_def)
-    apply(induction n)
-     apply(simp_all)
-    by(unat_arith)
-
-  lemma ipv4addr_of_nat_eq: "x = y \<Longrightarrow> ipv4addr_of_nat x = ipv4addr_of_nat y"
-    by(simp add: ipv4addr_of_nat_def)
-
-subsection\<open>Representing IPv4 Adresses\<close>
+subsection\<open>Representing IPv4 Adresses (Syntax)\<close>
   fun ipv4addr_of_dotdecimal :: "nat \<times> nat \<times> nat \<times> nat \<Rightarrow> ipv4addr" where
     "ipv4addr_of_dotdecimal (a,b,c,d) = ipv4addr_of_nat (d + 256 * c + 65536 * b + 16777216 * a )"
 
@@ -74,12 +54,18 @@ subsection\<open>Representing IPv4 Adresses\<close>
   declare ipv4addr_of_dotdecimal.simps[simp del]
   declare dotdecimal_of_ipv4addr.simps[simp del]
 
-  lemma "ipv4addr_of_dotdecimal (192, 168, 0, 1) = 3232235521" by eval
-  lemma "dotdecimal_of_ipv4addr 3232235521 = (192, 168, 0, 1)" by eval
+  text\<open>Examples:\<close>
+  lemma "ipv4addr_of_dotdecimal (192, 168, 0, 1) = 3232235521"
+    by(simp add: ipv4addr_of_dotdecimal.simps ipv4addr_of_nat_def)
+    (*could be solved by eval, but needs "~~/src/HOL/Library/Code_Target_Nat"*)
+  lemma "dotdecimal_of_ipv4addr 3232235521 = (192, 168, 0, 1)"
+    by(simp add: dotdecimal_of_ipv4addr.simps nat_of_ipv4addr_def)
 
   text\<open>a different notation for @{term ipv4addr_of_dotdecimal}\<close>
   lemma ipv4addr_of_dotdecimal_bit: 
-    "ipv4addr_of_dotdecimal (a,b,c,d) = (ipv4addr_of_nat a << 24) + (ipv4addr_of_nat b << 16) + (ipv4addr_of_nat c << 8) + ipv4addr_of_nat d"
+    "ipv4addr_of_dotdecimal (a,b,c,d) =
+      (ipv4addr_of_nat a << 24) + (ipv4addr_of_nat b << 16) +
+       (ipv4addr_of_nat c << 8) + ipv4addr_of_nat d"
   proof -
     have a: "(ipv4addr_of_nat a) << 24 = ipv4addr_of_nat (a * 16777216)"
       by(simp add: ipv4addr_of_nat_def shiftl_t2n)
@@ -90,93 +76,83 @@ subsection\<open>Representing IPv4 Adresses\<close>
     have ipv4addr_of_nat_suc: "\<And>x. ipv4addr_of_nat (Suc x) = word_succ (ipv4addr_of_nat (x))"
       by(simp add: ipv4addr_of_nat_def, metis Abs_fnat_hom_Suc of_nat_Suc)
     { fix x y
-    have "ipv4addr_of_nat x + ipv4addr_of_nat y = ipv4addr_of_nat (x+y)"
-      apply(induction x arbitrary: y)
-       apply(simp add: ipv4addr_of_nat_def)
-      apply(simp add: ipv4addr_of_nat_suc word_succ_p1)
-      done
+      have "ipv4addr_of_nat x + ipv4addr_of_nat y = ipv4addr_of_nat (x+y)"
+        apply(induction x arbitrary: y)
+         apply(simp add: ipv4addr_of_nat_def; fail)
+        by(simp add: ipv4addr_of_nat_suc word_succ_p1)
     } from this a b c
     show ?thesis
-    apply(simp add: ipv4addr_of_dotdecimal.simps)
-    apply(rule ipv4addr_of_nat_eq)
-    by presburger
+      apply(simp add: ipv4addr_of_dotdecimal.simps)
+      apply(rule arg_cong[where f=ipv4addr_of_nat])
+      apply(thin_tac _)+
+      by presburger
   qed
 
-
   lemma size_ipv4addr: "size (x::ipv4addr) = 32" by(simp add:word_size)
-  lemma "(4294967296::ipv4addr) = 2^32" by eval
-
-  lemma nat_of_ipv4addr_slice_ipv4addr_of_nat: 
-    "nat_of_ipv4addr (slice x (ipv4addr_of_nat a)) = (nat_of_ipv4addr (ipv4addr_of_nat a)) div 2^x"
-    proof -
-      have mod4294967296: "int a mod 4294967296 = int (a mod 4294967296)"
-        using zmod_int by auto
-      (*TODO: why is this gone in 2016?*)
-      have zpower_int: "\<And>m n. int m ^ n = int (m ^ n)" using of_nat_power by simp
-      have int_pullin: "int (a mod 4294967296) div 2 ^ x = int (a mod 4294967296 div 2 ^ x)"
-        using zpower_int zdiv_int by (metis of_nat_numeral) 
-    show ?thesis
-      apply(simp add: shiftr_slice[symmetric])
-      apply(simp add: ipv4addr_of_nat_def word_of_nat)
-      apply(simp add: nat_of_ipv4addr_def unat_def)
-      apply(simp add: shiftr_div_2n)
-      apply(simp add: uint_word_of_int)
-      apply(simp add: mod4294967296 int_pullin)
-      done
-     qed
-  lemma ipv4addr_and_255: "(x::ipv4addr) AND 255 = x AND mask 8"
-    by(simp add: mask_def)
-  lemma ipv4addr_of_nat_AND_mask8: "(ipv4addr_of_nat a) AND mask 8 = (ipv4addr_of_nat (a mod 256))"
-    apply(simp add: ipv4addr_of_nat_def and_mask_mod_2p)
-    apply(simp add: word_of_nat) (*use this to get rid of of_nat. All thm are with word_of_int*)
-    apply(simp add: uint_word_of_int)
-    apply(subst mod_mod_cancel)
-     apply simp
-    apply(simp add: zmod_int)
-    done
  
   lemma dotdecimal_of_ipv4addr_ipv4addr_of_dotdecimal:
-  "\<lbrakk> a < 256; b < 256; c < 256; d < 256 \<rbrakk> \<Longrightarrow> dotdecimal_of_ipv4addr (ipv4addr_of_dotdecimal (a,b,c,d)) = (a,b,c,d)"
+  "\<lbrakk> a < 256; b < 256; c < 256; d < 256 \<rbrakk> \<Longrightarrow>
+    dotdecimal_of_ipv4addr (ipv4addr_of_dotdecimal (a,b,c,d)) = (a,b,c,d)"
   proof -
     assume  "a < 256" and "b < 256" and "c < 256" and "d < 256"
     note assms= \<open>a < 256\<close> \<open>b < 256\<close> \<open>c < 256\<close> \<open>d < 256\<close> 
-    hence a: "nat_of_ipv4addr ((ipv4addr_of_nat (d + 256 * c + 65536 * b + 16777216 * a) >> 24) AND mask 8) = a"
+    hence a:  "nat_of_ipv4addr ((ipv4addr_of_nat (d + 256 * c + 65536 * b + 16777216 * a) >> 24) AND mask 8) = a"
       apply(simp add: ipv4addr_of_nat_def word_of_nat)
       apply(simp add: nat_of_ipv4addr_def unat_def)
       apply(simp add: and_mask_mod_2p)
       apply(simp add: shiftr_div_2n)
       apply(simp add: uint_word_of_int)
       apply(subst mod_pos_pos_trivial)
-        apply simp_all
+        apply(simp; fail)
+       apply(simp; fail)
+      apply(simp)
       apply(subst mod_pos_pos_trivial)
-        apply simp_all
+        apply(simp; fail)
+       apply(simp; fail)
       apply(subst mod_pos_pos_trivial)
-        apply simp_all
+        by simp+
+    have ipv4addr_of_nat_AND_mask8: "(ipv4addr_of_nat a) AND mask 8 = (ipv4addr_of_nat (a mod 256))"
+      for a
+      apply(simp add: ipv4addr_of_nat_def and_mask_mod_2p)
+      apply(simp add: word_of_nat) (*use this to get rid of of_nat. All thm are with word_of_int*)
+      apply(simp add: uint_word_of_int)
+      apply(subst mod_mod_cancel)
+       apply(simp; fail)
+      apply(simp add: zmod_int)
       done
-    from assms have b: "nat_of_ipv4addr ((ipv4addr_of_nat (d + 256 * c + 65536 * b + 16777216 * a) >> 16) AND mask 8) = b"
+    from assms have b:
+      "nat_of_ipv4addr ((ipv4addr_of_nat (d + 256 * c + 65536 * b + 16777216 * a) >> 16) AND mask 8) = b"
       apply(simp add: ipv4addr_of_nat_def word_of_nat)
       apply(simp add: nat_of_ipv4addr_def unat_def)
       apply(simp add: and_mask_mod_2p)
       apply(simp add: shiftr_div_2n)
       apply(simp add: uint_word_of_int)
       apply(subst mod_pos_pos_trivial)
-        apply simp_all
+        apply(simp; fail)
+       apply(simp; fail)
       apply(subst mod_pos_pos_trivial[where b="4294967296"])
-        apply simp_all
-      apply(simp add: NumberWang.div65536[simplified]) (*we add the simplified because the WordLemmaBucket adds some additional simp rules*)
+        apply(simp; fail)
+       apply(simp; fail)
+      apply(simp add: NumberWang.div65536[simplified])
+      (*The [simplified] is needed because Word_Lib adds some additional simp rules*)
       done
-      --\<open>When @{file "../Word_Lib/Word_Lemmas.thy"} is imported, some @{file "NumberWang.thy"} lemmas need the [simplified] attribute
-          because WordLemmaBucket adds some simp rules. This theory should also work without Word_Lemmas\<close>
-    from assms have c: "nat_of_ipv4addr ((ipv4addr_of_nat (d + 256 * c + 65536 * b + 16777216 * a) >> 8) AND mask 8) = c"
+      --\<open>When @{file "../Word_Lib/Word_Lemmas.thy"} is imported,
+         some @{file "NumberWang.thy"} lemmas need the [simplified] attribute
+         because @{text Word_Lib} adds some simp rules.
+         This theory should also work without @{file "../Word_Lib/Word_Lemmas.thy"}\<close>
+    from assms have c:
+      "nat_of_ipv4addr ((ipv4addr_of_nat (d + 256 * c + 65536 * b + 16777216 * a) >> 8) AND mask 8) = c"
       apply(simp add: ipv4addr_of_nat_def word_of_nat)
       apply(simp add: nat_of_ipv4addr_def unat_def)
       apply(simp add: and_mask_mod_2p)
       apply(simp add: shiftr_div_2n)
       apply(simp add: uint_word_of_int)
       apply(subst mod_pos_pos_trivial)
-        apply simp_all
+        apply(simp; fail)
+       apply(simp; fail)
       apply(subst mod_pos_pos_trivial[where b="4294967296"])
-        apply simp_all
+        apply(simp; fail)
+       apply(simp; fail)
       apply(simp add: NumberWang.div256[simplified])
       done
     from \<open>d < 256\<close> have d: "nat_of_ipv4addr (ipv4addr_of_nat (d + 256 * c + 65536 * b + 16777216 * a) AND mask 8) = d"
@@ -184,16 +160,12 @@ subsection\<open>Representing IPv4 Adresses\<close>
       apply(simp add: ipv4addr_of_nat_def word_of_nat)
       apply(simp add: nat_of_ipv4addr_def)
       apply(subgoal_tac "(d + 256 * c + 65536 * b + 16777216 * a) mod 256 = d")
-      prefer 2
-       apply(simp add: NumberWang.mod256)
-      apply(simp)
-      apply(simp add: unat_def)
-      apply(simp add: uint_word_of_int)
-      apply(simp add: mod_pos_pos_trivial)
+       apply(simp add: unat_def uint_word_of_int mod_pos_pos_trivial; fail)
+      apply(simp add: NumberWang.mod256)
       done
     from a b c d show ?thesis
       apply(simp add: ipv4addr_of_dotdecimal.simps dotdecimal_of_ipv4addr.simps)
-      apply(simp add: ipv4addr_and_255)
+      apply(simp add: mask_def)
       done
   qed
   
@@ -202,17 +174,15 @@ subsection\<open>Representing IPv4 Adresses\<close>
   proof -
     have ip_and_mask8_bl_drop24: "(ip::ipv4addr) AND mask 8 = of_bl (drop 24 (to_bl ip))"
       by(simp add: Word_Lemmas.of_drop_to_bl size_ipv4addr)
-  
-    have List_rev_drop_geqn: "\<And>x n. length x \<ge> n \<Longrightarrow> (take n (rev x)) = rev (drop (length x - n) x)"
-      by(simp add: List.rev_drop)
-  
-    have and_mask_bl_take: "\<And> x n. length x \<ge> n \<Longrightarrow> ((of_bl x) AND mask n) = (of_bl (rev (take n (rev (x)))))"
-      apply(simp add: List_rev_drop_geqn)
-      apply(simp add: Word_Lib.of_bl_drop)
-      done
-  
-    have bit_equality: "((ip >> 24) AND 0xFF << 24) + ((ip >> 16) AND 0xFF << 16) + ((ip >> 8) AND 0xFF << 8) + (ip AND 0xFF) =
-      of_bl (take 8 (to_bl ip) @ take 8 (drop 8 (to_bl ip)) @ take 8 (drop 16 (to_bl ip)) @ drop 24 (to_bl ip))"
+    have List_rev_drop_geqn: "length x \<ge> n \<Longrightarrow> (take n (rev x)) = rev (drop (length x - n) x)"
+      for x :: "'a list" and n by(simp add: List.rev_drop)
+    have and_mask_bl_take: "length x \<ge> n \<Longrightarrow> ((of_bl x) AND mask n) = (of_bl (rev (take n (rev (x)))))"
+      for x n by(simp add: List_rev_drop_geqn of_bl_drop)
+    have ipv4addr_and_255: "x AND 255 = x AND mask 8" for x :: ipv4addr
+      by(simp add: mask_def)
+    have bit_equality:
+      "((ip >> 24) AND 0xFF << 24) + ((ip >> 16) AND 0xFF << 16) + ((ip >> 8) AND 0xFF << 8) + (ip AND 0xFF) =
+       of_bl (take 8 (to_bl ip) @ take 8 (drop 8 (to_bl ip)) @ take 8 (drop 16 (to_bl ip)) @ drop 24 (to_bl ip))"
       apply(simp add: ipv4addr_and_255)
       apply(simp add: shiftr_slice)
       apply(simp add: Word.slice_take' size_ipv4addr)
@@ -223,94 +193,82 @@ subsection\<open>Representing IPv4 Adresses\<close>
       apply(simp add: of_bl_append)
       apply(simp add: ip_and_mask8_bl_drop24)
       done
-  
     have blip_split: "\<And> blip. length blip = 32 \<Longrightarrow>
       blip = (take 8 blip) @ (take 8 (drop 8 blip)) @ (take 8 (drop 16 blip)) @ (take 8 (drop 24 blip))"
-      apply(case_tac blip)
-      apply(simp_all)
-      (*thin_tac "blip = ?x",*)
-      apply(rename_tac blip,case_tac blip,simp_all)+ (*I'm so sorry for this ...*)
-      done
-  
+      by(rename_tac blip,case_tac blip,simp_all)+ (*I'm so sorry for this ...*)
     have "ipv4addr_of_dotdecimal (dotdecimal_of_ipv4addr ip) = of_bl (to_bl ip)"
       apply(subst blip_split)
-       apply(simp)
+       apply(simp; fail)
       apply(simp add: ipv4addr_of_dotdecimal_bit dotdecimal_of_ipv4addr.simps)
       apply(simp add: ipv4addr_of_nat_nat_of_ipv4addr)
       apply(simp add: bit_equality)
       done
-  
     thus ?thesis using Word.word_bl.Rep_inverse[symmetric] by simp
   qed
 
-
-  lemma ipv4addr_of_dotdecimal_eqE: "\<lbrakk> ipv4addr_of_dotdecimal (a,b,c,d) = ipv4addr_of_dotdecimal (e,f,g,h); a < 256; b < 256; c < 256; d < 256; e < 256; f < 256; g < 256; h < 256 \<rbrakk> \<Longrightarrow>
-     a = e \<and> b = f \<and> c = g \<and> d = h"
+  lemma ipv4addr_of_dotdecimal_eqE:
+    "\<lbrakk> ipv4addr_of_dotdecimal (a,b,c,d) = ipv4addr_of_dotdecimal (e,f,g,h);
+       a < 256; b < 256; c < 256; d < 256; e < 256; f < 256; g < 256; h < 256 \<rbrakk> \<Longrightarrow>
+         a = e \<and> b = f \<and> c = g \<and> d = h"
      by (metis Pair_inject dotdecimal_of_ipv4addr_ipv4addr_of_dotdecimal)
 
-
-subsection\<open>IP ranges\<close>
-  lemma UNIV_ipv4addrset: "(UNIV :: ipv4addr set) = {0 .. max_ipv4_addr}" by(auto)
-  lemma "(42::ipv4addr) \<in> UNIV" by eval
-
+subsection\<open>IP Ranges: Examples\<close>
+  lemma "(UNIV :: ipv4addr set) = {0 .. max_ipv4_addr}" by(simp add: UNIV_ipv4addrset)
+  lemma "(42::ipv4addr) \<in> UNIV" by(simp)
 
   (*Warning, not executable!*)
-  definition ipv4set_from_netmask::"ipv4addr \<Rightarrow> ipv4addr \<Rightarrow> ipv4addr set" where
-    "ipv4set_from_netmask addr netmask \<equiv> ipset_from_netmask addr netmask"
 
-
-  lemma "ipv4set_from_netmask (ipv4addr_of_dotdecimal (192,168,0,42)) (ipv4addr_of_dotdecimal (255,255,0,0)) =
+  lemma "ipset_from_netmask (ipv4addr_of_dotdecimal (192,168,0,42)) (ipv4addr_of_dotdecimal (255,255,0,0)) =
           {ipv4addr_of_dotdecimal (192,168,0,0) .. ipv4addr_of_dotdecimal (192,168,255,255)}"
-   by(simp add: ipv4set_from_netmask_def ipset_from_netmask_def ipv4addr_of_dotdecimal.simps ipv4addr_of_nat_def)
+   by(simp add: ipset_from_netmask_def ipv4addr_of_dotdecimal.simps ipv4addr_of_nat_def)
 
-  lemma "ipv4set_from_netmask (ipv4addr_of_dotdecimal (192,168,0,42)) (ipv4addr_of_dotdecimal (0,0,0,0)) = UNIV"
-    by(simp add: UNIV_ipv4addrset ipset_from_netmask_def ipv4addr_of_dotdecimal.simps ipv4addr_of_nat_def ipv4set_from_netmask_def max_ipv4_addr_max_word)
-   
+  lemma "ipset_from_netmask (ipv4addr_of_dotdecimal (192,168,0,42)) (ipv4addr_of_dotdecimal (0,0,0,0)) = UNIV"
+    by(simp add: UNIV_ipv4addrset ipset_from_netmask_def ipv4addr_of_dotdecimal.simps
+                 ipv4addr_of_nat_def max_ipv4_addr_max_word)
   
   text\<open>192.168.0.0/24\<close>
-  definition ipv4set_from_cidr::"ipv4addr \<Rightarrow> nat \<Rightarrow> ipv4addr set" where
-    "ipv4set_from_cidr addr pflength \<equiv> ipset_from_cidr addr pflength"
 
-  lemma ipv4set_from_cidr_alt: "ipv4set_from_cidr addr pflength = ipv4set_from_netmask addr ((mask pflength) << (32 - pflength))"
-    by(simp add: ipv4set_from_cidr_def ipv4set_from_netmask_def ipset_from_cidr_def)
+  lemma fixes addr :: ipv4addr
+    shows "ipset_from_cidr addr pflength =
+            ipset_from_netmask addr ((mask pflength) << (32 - pflength))"
+    by(simp add: ipset_from_cidr_def)
 
-  lemma "ipv4set_from_cidr (ipv4addr_of_dotdecimal (192,168,0,42)) 16 = 
+  lemma "ipset_from_cidr (ipv4addr_of_dotdecimal (192,168,0,42)) 16 = 
           {ipv4addr_of_dotdecimal (192,168,0,0) .. ipv4addr_of_dotdecimal (192,168,255,255)}"
-   by(simp add: ipv4set_from_cidr_def ipset_from_cidr_alt mask_def  ipv4addr_of_dotdecimal.simps ipv4addr_of_nat_def)
+   by(simp add: ipset_from_cidr_alt mask_def  ipv4addr_of_dotdecimal.simps ipv4addr_of_nat_def)
 
-  lemma ipv4set_from_cidr_0: "ipv4set_from_cidr foo 0 = UNIV"
-    by(simp add: ipv4set_from_cidr_def ipset_from_cidr_0)
+  lemma "ip \<in> (ipset_from_cidr (ipv4addr_of_dotdecimal (0, 0, 0, 0)) 0)"
+    by(simp add: ipset_from_cidr_0)
 
-  lemma "ipv4set_from_cidr 0 0 = UNIV"
-    by(simp add: ipv4set_from_cidr_def ipset_from_cidr_0)
-  lemma "ip \<in> (ipv4set_from_cidr (ipv4addr_of_dotdecimal (0, 0, 0, 0)) 0)"
-    by(simp add: ipv4set_from_cidr_0)
+  lemma ipv4set_from_cidr_32: fixes addr :: ipv4addr
+    shows "ipset_from_cidr addr 32 = {addr}"
+    by(simp add: ipset_from_cidr_alt mask_def)
 
-  lemma ipv4set_from_cidr_32: "ipv4set_from_cidr foo 32 = {foo}"
-    by(simp add: ipv4set_from_cidr_alt ipv4set_from_netmask_def mask_def ipset_from_netmask_minusone)
-
-  (*TODO: delete completely, use generic version*)
-  lemma "ipv4set_from_cidr pre len = {(pre AND ((mask len) << (32 - len))) .. pre OR (mask (32 - len))}"
-    by (simp add: ipset_from_cidr_alt ipv4set_from_cidr_def)
-
+  lemma  fixes pre :: ipv4addr
+    shows "ipset_from_cidr pre len = {(pre AND ((mask len) << (32 - len))) .. pre OR (mask (32 - len))}"
+    by (simp add: ipset_from_cidr_alt ipset_from_cidr_def)
 
   text\<open>making element check executable\<close>
   lemma addr_in_ipv4set_from_netmask_code[code_unfold]: 
-    "addr \<in> (ipv4set_from_netmask base netmask) \<longleftrightarrow> (base AND netmask) \<le> addr \<and> addr \<le> (base AND netmask) OR (NOT netmask)"
-    by (simp add: addr_in_ipset_from_netmask_code ipv4set_from_netmask_def)
-  lemma addr_in_ipv4set_from_cidr_code[code_unfold]: "addr \<in> (ipv4set_from_cidr pre len) \<longleftrightarrow> 
+    fixes addr :: ipv4addr
+    shows "addr \<in> (ipset_from_netmask base netmask) \<longleftrightarrow>
+            (base AND netmask) \<le> addr \<and> addr \<le> (base AND netmask) OR (NOT netmask)"
+    by (simp add: addr_in_ipset_from_netmask_code)
+  lemma addr_in_ipv4set_from_cidr_code[code_unfold]: 
+    fixes addr :: ipv4addr
+    shows "addr \<in> (ipset_from_cidr pre len) \<longleftrightarrow> 
               (pre AND ((mask len) << (32 - len))) \<le> addr \<and> addr \<le> pre OR (mask (32 - len))"
-    by(simp add: ipv4set_from_cidr_def addr_in_ipset_from_cidr_code)
+    by(simp add: addr_in_ipset_from_cidr_code)
 
-  value[code] "ipv4addr_of_dotdecimal (192,168,4,8) \<in> (ipv4set_from_cidr (ipv4addr_of_dotdecimal (192,168,0,42)) 16)"
+  (*small numbers because we didn't load Code_Target_Nat*)
+  lemma "ipv4addr_of_dotdecimal (0,0,0,8) \<in> (ipset_from_cidr (ipv4addr_of_dotdecimal (0,0,0,0)) 16)"
+    by eval
 
-  
   definition ipv4range_UNIV :: "32 wordinterval" where "ipv4range_UNIV \<equiv> wordinterval_UNIV"
   
   lemma ipv4range_UNIV_set_eq: "wordinterval_to_set ipv4range_UNIV = UNIV"
     by(simp only: ipv4range_UNIV_def wordinterval_UNIV_set_eq)
  
-
 
   thm iffD1[OF wordinterval_eq_set_eq]
   (*TODO: probably the following is a good idea?*)
